

$$\max \quad Z = -2x_1 - x_2 \quad x_1, x_2 \geq 0$$

$$\text{s.t.} \quad \left. \begin{array}{l} -x_1 + x_2 \leq -1 \\ -x_1 - 2x_2 \leq -2 \\ x_2 \leq 1 \end{array} \right\} \text{origin is not feasible}$$

Auxiliary Problem

$$\max \quad Z = -x_0$$

$$\text{s.t.} \quad -x_1 + x_2 - x_0 \leq -1 \quad x_1, x_2, x_0 \geq 0$$

$$-x_1 - 2x_2 - x_0 \leq -2$$

$$(1) \text{ must be feasible: } x_2 - x_0 \leq 1$$

choose x_0 large enough

(2) Original problem is feasible

$$\Leftrightarrow \max Z = 0 \quad (\text{Note: } \max Z \leq 0)$$

$$\max \quad Z = -x_0$$

$$\text{s.t.} \quad w_1 = -1 - x_1 - x_2 + x_0$$

$$w_2 = -2 + x_1 + 2x_2 + x_0$$

$$w_3 = 1 - x_2 + x_0$$

$$\text{Set } x_1, x_2, x_0 = 0 \Rightarrow \begin{array}{l} w_1 = -1 \quad \text{bc } w_1, w_2 < 0 \\ w_2 = -2 \quad \leftarrow \text{most infeasible} \\ w_3 = 1 \quad \quad \quad (\text{interchange } x_0 \text{ \& } w_2) \end{array}$$

$$\max \quad z = -x_0$$

$$\text{s.t.} \quad w_1 = -1 - x_1 - x_2 + x_0$$

$$w_2 = -2 + x_1 + 2x_2 + x_0$$

$$w_3 = 1 - x_2 + x_0$$



$$x_0 = w_2 + 2 - x_1 - 2x_2$$

↓ insert x_0 in w_1 and w_3 and simplify

$$w_1 = 1 - 3x_2 + w_2$$

$$w_3 = 3 - x_1 - 3x_2 + w_2$$

①

$$z = -x_0$$

$$\max \quad z = -2 + x_1 + \underline{\underline{2x_2 - w_2}}$$

$$\text{s.t.} \quad x_0 = 2 - x_1 - 2x_2 + w_2, \quad x_0 = 2 - 2x_2 \geq 0$$

$$w_1 = 1 - 3x_2 + w_2, \quad w_1 = 1 - 3x_2 \geq 0$$

$$w_3 = 3 - x_1 - 3x_2 + w_2, \quad w_3 = 3 - 3x_2 \geq 0$$

$$\begin{array}{l} \text{Set } x_1, x_2, w_2 = 0 \Rightarrow \\ \text{pick } x_2 \text{ highest coeff} \end{array} \quad \left. \begin{array}{l} x_0 = 2 \\ w_1 = 1 \\ w_3 = 3 \end{array} \right\} \begin{array}{l} \text{feasible set!} \\ \text{bc basic vars} \geq 0 \end{array}$$

$$x_0: -2x_2 \geq -2 \Rightarrow x_2 \leq 1$$

$$w_1: -3x_2 \geq -1 \Rightarrow x_2 \leq 1/3 \leftarrow \text{pick tightest}$$

$$w_3: -3x_2 \geq -3 \Rightarrow x_2 \leq 1$$

so interchange x_2, w_1

$$x_2 = \frac{1}{3} - \frac{w_1}{3} + \frac{w_2}{3} \quad (\text{sub into } x_0, w_3)$$

$$w_3 = 2 - x_1 + w_1$$

$$x_0 = \frac{4}{3} - x_1 + \frac{2}{3} w_1 + \frac{1}{3} w_2$$

$$\max \quad z = -\frac{4}{3} + x_1 - \frac{2}{3} w_1 - \frac{w_2}{3}$$

↑ Increase

$$x_2 = \frac{1}{3} - \frac{1}{3} w_1 + \frac{1}{3} w_2$$

$$\text{s.t.} \quad w_3 = 2 - x_1 + w_1$$

$$x_0 = \frac{4}{3} - x_1 + \frac{2}{3} w_1 + \frac{1}{3} w_2$$

x_2 : Does not have x_1

$$w_3: w_3 = 2 - x_1 \geq 0 \Rightarrow 2 \geq x_1$$

$$x_0: x_0 = \frac{4}{3} - x_1 \geq 0 \Rightarrow \frac{4}{3} \geq x_1 \leftarrow \text{tightest bound}$$

change x_0, x_1

$$x_0 - \frac{4}{3} - \frac{2}{3} w_1 - \frac{1}{3} w_2 = -x_1 \leftarrow \text{sub back}$$

$$x_1 = \frac{4}{3} + \frac{2}{3} w_1 + \frac{1}{3} w_2 - x_0$$

$$x_2 = \frac{1}{3} - \frac{1}{3} w_1 + \frac{1}{3} w_2$$

$$w_3 = \frac{2}{3} + \frac{1}{3} w_1 - \frac{1}{3} w_2 + x_1$$

$$z = -\frac{4}{3} + \left(\frac{4}{3} + \frac{2}{3} w_1 + \frac{1}{3} w_2 - x_0 \right) - \frac{2}{3} w_1 - \frac{w_2}{3}$$

$$z = -x_0$$

$$\text{s.t.} \quad x_1 = \frac{4}{3} + \frac{2}{3} w_1 + \frac{1}{3} w_2 - x_0$$

$$w_3 = \frac{2}{3} + \frac{1}{3} w_1 - \frac{1}{3} w_2 + x_0$$

$$x_2 = \frac{1}{3} - \frac{1}{3} w_1 + \frac{1}{3} w_2$$

$$\text{Set } w_1, w_2, x_0 = 0 \Rightarrow \left. \begin{array}{l} x_1 = 4/3 \\ w_3 = 2/3 \\ x_2 = 1/3 \end{array} \right\} \text{ optimal!}$$

Back to OG Problem

$$\max z = -2x_1 - x_2$$

$$\text{s.t.} \quad -x_1 + x_2 \leq 1 \quad x_1, x_2 \geq 0$$

$$-x_1 - 2x_2 \leq -2$$

$$x_2 \leq 1$$

$$z = -2 \left(\frac{4}{3} + \frac{2}{3} w_1 + \frac{1}{3} w_2 \right) - \left(\frac{1}{3} - \frac{1}{3} w_1 + \frac{1}{3} w_2 \right)$$

$$= -3 - w_1 - w_2 \quad \text{and } w_1 = w_2 = 0 \text{ so already optimal}$$